Modified lowenheim's formula

B-unification/lowenheim.v
@@ -13,71 +13,54 @@ Require Export terms.
 Require Import List.
 Import ListNotations.
 
-
 (** LOWENHEIM'S FORMULA **)
 
-(* Maps boolean number to term *)
-Definition tau (b : bool) : term :=
-  match b with
-    | false => T0
-    | true  => T1
+(* Generates a lowenheim replacement *)
+Definition lowenheim_replace (t : term) (r : replacement) : replacement :=
+  if term_contains_var t (fst r) then 
+    (fst r, (t + T1) * VAR (fst r) + t * (snd r))
+  else
+    (fst r, VAR (fst r)).
+
+(* Builds a lowenheim substitution for a given term from a substitution *)
+Fixpoint lowenheim_subst (t : term) (sigma : subst) : subst :=
+  match sigma with
+    | nil => nil
+    | r :: s' => (lowenheim_replace t r) :: (lowenheim_subst t s')
   end.
 
-(* Creates a single replacement (var -> term) for lowenheim's formula *)
-Definition lowenheim_replace (t : term) (v : var) (b : bool) : replacement :=
-  (v, (t + T1) * VAR v + t * (tau b)).
-
-(* Creates a substitution (list replacement) for lowenheim's formula. Any variables entered into vars will be 
-   set to 1 *)
-Fixpoint lowenheim_subst (t : term) (term_vars : var_set) (vars : var_set) : subst :=
-  match term_vars with (* Ensure term_vars is unique *)
-    | nil => nil (* Can't create a substitution for a term with no variables! *)
-    | v :: v' => (lowenheim_replace t v (var_set_includes_var v vars)) :: (lowenheim_subst t v' vars)
-  end.
-
-(* Lowenheim's formula *)
-Definition lowenheim (t : term) (vars : var_set) : subst :=
-  lowenheim_subst t (term_unique_vars t) vars.
-
-Example lowenheim_ex1 :
-  mgu (VAR 0 * VAR 1) (lowenheim (VAR 0 * VAR 1) ([0; 1])).
+Example lowenheim_subst_ex1 :
+  (unifier (VAR 0 * VAR 1) (lowenheim_subst (VAR 0 * VAR 1) ((0, T1) :: (1, T0) :: nil))).
 Proof.
-unfold mgu. intros. unfold lowenheim. simpl in *.
-unfold more_general_subst. intros. unfold lowenheim_replace. simpl.
-inversion H.
+unfold unifier. unfold lowenheim_subst. simpl. 
+rewrite mul_comm with (y := T0). rewrite mul_T0_x.
+rewrite sum_comm with (y := T0). rewrite sum_id.
+rewrite mul_comm with (y := T1). rewrite mul_id.
+rewrite mul_comm with (y := VAR 0). 
+rewrite mul_comm with (y := VAR 1).
+rewrite distr with (x := VAR 1). rewrite mul_comm with (y := T1).
+rewrite mul_id. rewrite mul_comm with (y := VAR 1).
+rewrite <- mul_assoc with (y := VAR 1) (z := VAR 0).
+rewrite mul_x_x. rewrite distr with (x := VAR 0) (y := VAR 1 * VAR 0).
+rewrite mul_comm with (y := VAR 0). rewrite <- mul_assoc with (y := VAR 0).
+rewrite mul_x_x. rewrite sum_x_x. rewrite sum_id. rewrite sum_comm.
+rewrite sum_id. rewrite mul_comm with (y := T1). rewrite mul_id.
+rewrite distr. rewrite <- mul_assoc with (y := VAR 0).
+rewrite mul_x_x. rewrite sum_x_x. reflexivity.
 Qed.
 
-Example lowenheim_ex2 :
-  mgu (VAR 0 * VAR 1) (lowenheim (VAR 0 * VAR 1) ([0])).
+Lemma lowenheim_subst_generates_unifiers :
+  forall (t : term) (sigma : subst) , unifier t sigma -> unifier t (lowenheim_subst t sigma).
 Proof.
-unfold mgu. intros. unfold lowenheim. simpl in *.
-unfold more_general_subst. intros. unfold lowenheim_replace. simpl.
-inversion H.
-Qed.
+intro. induction sigma.
+{
+  simpl in *. intros. apply H.
+}
+{
+  apply unifier_subset_imply_superset with (r := a) in IHsigma.
+  {
+Admitted.
 
-Example lowenheim_ex3 :
-  mgu (VAR 0 * VAR 1) (lowenheim (VAR 0 * VAR 1) ([1])).
-Proof.
-unfold mgu. intros. unfold lowenheim. simpl in *.
-unfold more_general_subst. intros. unfold lowenheim_replace. simpl.
-inversion H.
-Qed.
-
-Example lowenheim_ex4 :
-  mgu (VAR 0 * VAR 1) (lowenheim (VAR 0 * VAR 1) ([])).
-Proof.
-unfold mgu. intros. unfold lowenheim. simpl in *.
-unfold more_general_subst. intros. unfold lowenheim_replace. simpl.
-inversion H.
-Qed.
-
-Example lowenheim_ex4 :
-  mgu (VAR 0 * VAR 1) (lowenheim (VAR 0 * VAR 1) ([])).
-Proof.
-unfold mgu. intros. unfold lowenheim. simpl in *.
-unfold more_general_subst. intros. unfold lowenheim_replace. simpl.
-inversion H.
-Qed.
 
 (* check that the input given to lowenheim is actually a ground solutions *)
 Definition check_correct_input (t : term)(vars : var_set) : bool := 
